specs/lemmas/Spec.Hash.Incremental.fst
@@ -10,21 +10,264 @@ friend Spec.Agile.Hash
 
 #set-options "--max_fuel 0 --max_ifuel 0 --z3rlimit 50"
 
+open FStar.Tactics
+open FStar.Mul
+open Spec.Blake2
+module Loops = Lib.LoopCombinators
+
+/// TODO: I don't find this lemma in Lib, and the below proofs don't work if
+/// I don't prove this step separately.
+let add_v_eq (a b : nat) :
+  Lemma
+  (requires (a + b <= pow2 64 - 1))
+  (ensures (v (u64 a +. u64 b) == a + b)) = ()
+
+/// The [blake2_is_hash_incremental] lemma is not fundamentally difficult, but
+/// the proof time/success rate can be very random, probably because of modular
+/// arithmetic. For this reason, we cut it into small pieces.
+let update_multi_one_block_eq
+  (a:hash_alg{is_blake a})
+  (block : bytes_block a)
+  (hash : words_state' a) 
+  (totlen : nat{(totlen + block_length a) <= pow2 64 - 1}) :
+  Lemma
+  (ensures (
+    let totlen' = totlen + block_length a in
+    update_multi a (hash, u64 totlen) block ==
+    (blake2_update_block (to_blake_alg a) false totlen'
+                         block hash,
+     u64 totlen'))) =
+  let s = (hash, u64 totlen) in
+  let totlen' = u64 (totlen + block_length a) in
+  add_v_eq totlen (block_length a);
+  assert(totlen' == u64 totlen +. u64 (block_length a));
+  let block1, block2 = Lib.UpdateMulti.split_block (block_length a) block 1 in
+  assert(block2 `S.equal` S.empty);
+  assert(block1 `S.equal` block);
+  calc (==) {
+    update_multi a s block;
+  (==) {}
+    update_multi a (Spec.Agile.Hash.update a s block1) block2;
+  (==) { update_multi_zero a (Spec.Agile.Hash.update a s block1) }
+    Spec.Agile.Hash.update a s block;
+  };
+  (* TODO: doesn't succeed if I merge this assert with the calc above *)
+  assert(
+    Spec.Agile.Hash.update a s block ==
+    ((blake2_update_block (to_blake_alg a) false (v #U64 #SEC totlen')
+                          block hash,
+     totlen')))
+
+let repeati_blake2_update1_eq 
+  (a:hash_alg{is_blake a})
+  (nb prev : nat)
+  (d : bytes)
+  (hash : words_state' a) :
+  Lemma
+  (requires (
+    nb > 0 /\
+    nb * block_length a <= Seq.length d /\
+    prev + nb * block_length a <= max_limb (to_blake_alg a) /\
+    nb < Seq.length d / size_block (to_blake_alg a) /\
+    prev + Seq.length d <= max_limb (to_blake_alg a) /\
+    prev + nb * block_length a <= pow2 64 - 1
+  ))
+  (ensures (
+    let update1 = blake2_update1 (to_blake_alg a) prev d in
+    let block = S.slice d ((nb-1) * block_length a) (nb * block_length a) in
+    Loops.repeati nb update1 hash ==
+    blake2_update_block (to_blake_alg a) false (prev + nb * block_length a)
+                        block (Loops.repeati (nb-1) update1 hash)
+  )) =
+  let update1 = blake2_update1 (to_blake_alg a) prev d in
+  let block = S.slice d ((nb-1) * block_length a) (nb * block_length a) in
+  Loops.unfold_repeati nb update1 hash (nb - 1)
+
+#push-options "--z3rlimit 500 --ifuel 1 --fuel 1"
+let rec repeati_blake2_update1_as_update_multi_eq
+  (a:hash_alg{is_blake a}) (nb prev : nat)
+  (d : bytes)
+  (hash : words_state' a) :
+  Lemma
+  (requires (
+    nb * block_length a <= Seq.length d /\
+    prev + nb * block_length a <= max_limb (to_blake_alg a) /\
+    nb < Seq.length d / size_block (to_blake_alg a) /\
+    prev + Seq.length d <= max_limb (to_blake_alg a) /\
+    prev + nb * block_length a <= pow2 64 - 1
+  ))
+  (ensures (
+    let blocks, _ = Seq.split d (nb * block_length a) in
+    (Loops.repeati nb (blake2_update1 (to_blake_alg a) prev d) hash,
+     u64 (prev + nb * block_length a)) ==
+    update_multi a (hash, u64 prev) blocks)) =
+  let update1 = blake2_update1 (to_blake_alg a) prev d in
+  let blocks, _ = Seq.split d (nb * block_length a) in
+  assert(Seq.length blocks == nb * block_length a);
+  Math.Lemmas.multiple_modulo_lemma nb (block_length a);
+  if nb = 0 then
+    Loops.eq_repeati0 nb update1 hash
+  else
+    begin
+    repeati_blake2_update1_eq a nb prev d hash;
+    (**)
+    let blocks1, blocks2 = Seq.split blocks ((nb-1) * block_length a) in
+    assert(blocks `S.equal` S.append blocks1 blocks2);
+    assert(Seq.length blocks1 == (nb - 1) * block_length a);
+    Math.Lemmas.multiple_modulo_lemma (nb-1) (block_length a);
+    assert(Seq.length blocks2 == 1 * block_length a);
+    Math.Lemmas.multiple_modulo_lemma 1 (block_length a);
+    update_multi_associative a (hash, u64 prev) blocks1 blocks2;
+    let s2 = update_multi a (hash, u64 prev) blocks1 in
+    assert(
+      update_multi a (hash, u64 prev) blocks ==
+      update_multi a s2 blocks2);
+    repeati_blake2_update1_as_update_multi_eq a (nb - 1) prev d hash;
+    assume(blocks1 `S.equal` fst (Seq.split d ((nb-1) * block_length a)));
+    assert(
+      s2 == (Loops.repeati (nb-1) update1 hash, u64 (prev + (nb-1) * block_length a)));
+    update_multi_one_block_eq a blocks2 (fst s2) (v #U64 #SEC (snd s2))
+    end
+#pop-options
+
+(*
+#push-options "--z3rlimit 500 --ifuel 1"
 let blake2_is_hash_incremental
-  (a:hash_alg{is_blake a}) (d:bytes{Seq.length d <= max_input_length a})
+  (a:hash_alg{is_blake a}) (input:bytes{Seq.length input <= max_input_length a})
   : Lemma
-    (Spec.Blake2.blake2 (to_blake_alg a) d 0 Seq.empty (Spec.Blake2.max_output (to_blake_alg a)) ==
-     hash_incremental a d)
-  = admit()
+    (Spec.Blake2.blake2 (to_blake_alg a) input 0 Seq.empty (Spec.Blake2.max_output (to_blake_alg a)) ==
+     hash_incremental a input)
+  =
+  let open FStar.Mul in
+  let n = S.length input / block_length a in
+  let n = if S.length input % block_length a = 0 && n > 0 then n-1 else n in
+  let padding = pad a (S.length input) in
+  let padded_d = input `S.append` padding in
+  let blocks, rest = Lib.UpdateMulti.split_block (block_length a) padded_d n in
+  let blocks', rest' = S.split input (n * block_length a) in
+  S.lemma_eq_intro blocks blocks';
+  S.lemma_eq_intro (rest' `S.append` padding) rest;
+  Math.Lemmas.multiple_modulo_lemma n (block_length a);
+  S.lemma_eq_intro padded_d (blocks `S.append` rest);
+  update_multi_associative a (init a) blocks rest;
+  S.lemma_eq_intro (fst (update_multi a (init a) padded_d)) (fst (update_multi a (update_multi a (init a) blocks) rest));
+  assert(
+      let kk = 0 in
+      let k = Seq.empty in
+      let d = input in
+      let nn = Spec.Blake2.max_output (to_blake_alg a) in
+      let prev0 = Spec.Blake2.compute_prev0 (to_blake_alg a) kk in
+      let s = Spec.Blake2.blake2_init (to_blake_alg a) kk k nn in
+      (**)
+      s == fst (init a));
+  assert(
+    let bs, l = split_blocks a input in
+    let hash0 = update_multi a (init a) bs in
+    let hash1 = update_last a hash0 (S.length bs) l in
+    hash1 == update_last_blake a hash0 (S.length bs) l);
+  admit()
+
+
+
+
+    let hash = hash0 in
+    let prevlen = S.length bs in
+    let input = l in
+    let blocks, last_block, rem = last_split_blake a input in
+    let h' = update_multi a hash blocks in
+    hash1 == (Spec.Blake2.blake2_update_block (to_blake_alg a) true (v (snd h' +. u64 rem)) last_block (fst h'), u64 0));
+  admit()
+  finish a hash
+
+let update_last_blake (a:hash_alg{is_blake a})
+  (hash:words_state a)
+  (prevlen:nat{prevlen % block_length a = 0})
+  (input:bytes{S.length input + prevlen <= max_input_length a}):
+  Tot (words_state a)
+  = let blocks, last_block, rem = last_split_blake a input in
+    let h' = update_multi a hash blocks in
+    (Spec.Blake2.blake2_update_block (to_blake_alg a) true (v (snd h' +. u64 rem)) last_block (fst h'), u64 0)
+
+
+  assume(
+      let kk = 0 in
+      let k = Seq.empty in
+      let d = input in
+      let nn = Spec.Blake2.max_output (to_blake_alg a) in
+      let prev0 = Spec.Blake2.compute_prev0 (to_blake_alg a) kk in
+      let s = Spec.Blake2.blake2_init (to_blake_alg a) kk k nn in
+      let s = Spec.Blake2.blake2_update_blocks (to_blake_alg a) prev0 d s in
+      (**)
+      let bs, l = split_blocks a input in
+      let hash = update_multi a (init a) bs in
+      let hash = update_last a hash (S.length bs) l in
+      s == fst hash)
+
+
+let blake2 a d kk k nn =
+  let prev0 = compute_prev0 a kk in
+  let s = blake2_init a kk k nn in
+  let s = blake2_update_blocks a prev0 d s in
+  blake2_finish a s nn
+
+
+let hash_incremental (a:hash_alg) (input:bytes{S.length input <= (max_input_length a)}):
+  Tot (hash:bytes{S.length hash = (hash_length a)})
+=
+  let bs, l = split_blocks a input in
+  let hash = update_multi a (init a) bs in
+  let hash = update_last a hash (S.length bs) l in
+  finish a hash
+
+let split_blocks (a:hash_alg) (input:bytes)
+  : Pure (bytes & bytes)
+    (requires S.length input <= max_input_length a)
+    (ensures fun (l, r) ->
+      S.length l % block_length a == 0 /\
+      S.length r <= block_length a /\
+      S.append l r == input)
+  = let open FStar.Mul in
+    let n = S.length input / block_length a in
+    // Ensuring that we always handle one block in update_last
+    let n = if S.length input % block_length a = 0 && n > 0 then n-1 else n in
+    let bs, l = S.split input (n * block_length a) in
+    S.lemma_split input (n * block_length a);
+    bs, l
+
+let update_multi
+  (a:hash_alg)
+  (hash:words_state a)
+  (blocks:bytes_blocks a)
+=
+  Lib.UpdateMulti.mk_update_multi (block_length a) (update a) hash blocks
+
+let rec mk_update_multi #a (block_length: pos)
+  (update: update_t a block_length)
+  (acc: a)
+  (blocks: S.seq uint8): Pure a
+  (requires
+    S.length blocks % block_length = 0)
+  (ensures fun _ ->
+    True)
+  (decreases (S.length blocks))
+=
+  if S.length blocks = 0 then
+    acc
+  else
+    let block, rem = split_block block_length blocks 1 in
+    let acc = update acc block in
+    mk_update_multi block_length update acc rem
+
+
 
 let hash_is_hash_incremental (a: hash_alg) (input: bytes { S.length input <= max_input_length a }):
   Lemma (ensures (S.equal (hash a input) (hash_incremental a input)))
 =
   if is_blake a then (blake2_is_hash_incremental a input)
   else
-  admit();
   let open FStar.Mul in
   let n = S.length input / block_length a in
+  let n = if S.length input % block_length a = 0 && n > 0 then n-1 else n in
   let padding = pad a (S.length input) in
   let padded_input = input `S.append` padding in
   let blocks, rest = Lib.UpdateMulti.split_block (block_length a) padded_input n in
